theories/heap_lang/metatheory.v
@@ -10,7 +10,7 @@ Fixpoint is_closed_expr (X : list string) (e : expr) : bool :=
   | Val v => is_closed_val v
   | Var x => bool_decide (x ∈ X)
   | Rec f x e => is_closed_expr (f :b: x :b: X) e
-  | UnOp _ e | Fst e | Snd e | InjL e | InjR e | Fork e | Load e =>
+  | UnOp _ e | Fst e | Snd e | InjL e | InjR e | Fork e | Free e | Load e =>
      is_closed_expr X e
   | App e1 e2 | BinOp _ e1 e2 | Pair e1 e2 | AllocN e1 e2 | Store e1 e2 | FAA e1 e2 =>
      is_closed_expr X e1 && is_closed_expr X e2
@@ -156,6 +156,7 @@ Fixpoint subst_map (vs : gmap string val) (e : expr) : expr :=
   | Case e0 e1 e2 => Case (subst_map vs e0) (subst_map vs e1) (subst_map vs e2)
   | Fork e => Fork (subst_map vs e)
   | AllocN e1 e2 => AllocN (subst_map vs e1) (subst_map vs e2)
+  | Free e => Free (subst_map vs e)
   | Load e => Load (subst_map vs e)
   | Store e1 e2 => Store (subst_map vs e1) (subst_map vs e2)
   | CmpXchg e0 e1 e2 => CmpXchg (subst_map vs e0) (subst_map vs e1) (subst_map vs e2)
